\documentclass{article}
\usepackage{ifthen}
\usepackage{epsfig}
\usepackage{newunicodechar}
  \newunicodechar{⁻}{${}^{-}$}% Superscript minus
  \newunicodechar{²}{${}^{2}$}% Superscript two
  \newunicodechar{³}{${}^{3}$}% Superscript three

\pagestyle{empty}
\begin{document}
${\bf r}_{i}$
\pagebreak

$0 \leq i < 3$
\pagebreak

\[ {\bf b}_{1} \equiv {\bf r}_{1} - {\bf r}_{0} \quad\quad\quad\quad {\bf b}_{2} \equiv {\bf r}_{2} - {\bf r}_{1} \]
\pagebreak

$\theta$
\pagebreak

\[ \cos(\theta) = \frac{{\bf b}_{1} \cdot {\bf b}_{2}} {|{\bf b}_{1}||{\bf b}_{2}|} \]
\pagebreak

$\theta = 0$
\pagebreak

$\cos(\theta)$
\pagebreak

\[ V(\theta) = \kappa [ 1 - \cos(\theta) ] \]
\pagebreak

$\kappa$
\pagebreak

$\theta_{0}$
\pagebreak

\[ V(\theta) = \frac{\kappa}{2} [ \cos(\theta) - \cos(\theta_0)]^{2} \]
\pagebreak

\[ V(\theta) = \frac{\kappa}{2} ( \theta - \theta_0 )^{2} \]
\pagebreak

$\theta_0$
\pagebreak

$V(r)$
\pagebreak

$r$
\pagebreak

\[ V(r) = \frac{1}{2}\kappa R_{0}^{2} \ln \left ( 1 - \frac{r^{2}}{R_{0}^{2}} \right ) \]
\pagebreak

$r_{c}$
\pagebreak

$dV(r))/dr$
\pagebreak

$f_{c}$
\pagebreak

$r > r_{c}$
\pagebreak

\[ V(r) = V(r_c) + f_{c}(r - r_{c}) \]
\pagebreak

$r_{0}$
\pagebreak

$R_{0}$
\pagebreak

\[ V(r) = \frac{\kappa}{2} ( r - l )^{2} \]
\pagebreak

$\epsilon$
\pagebreak

$l$
\pagebreak

\[ V(r) = \frac{\kappa}{2} r^{2} \]
\pagebreak

$q_{1}$
\pagebreak

$q_{2}$
\pagebreak

\[ V(r) = \frac{1}{4 \pi \epsilon r } {\rm erfc}( \alpha r) \]
\pagebreak

$ r < r_{c} $
\pagebreak

$V(r) = 0$
\pagebreak

$\alpha$
\pagebreak

$\cos(\phi)$
\pagebreak

$\phi$
\pagebreak

\[ V(\phi) = \kappa [ 1 + \cos(\phi) ] \]
\pagebreak

\[ V(\phi) = kappa [1 + cos(phi)] \]
\pagebreak

\[ {\bf b}_{1} \equiv {\bf r}_{1} - {\bf r}_{0} \quad\quad\quad {\bf b}_{2} \equiv {\bf r}_{2} - {\bf r}_{1} \quad\quad\quad {\bf b}_{3} \equiv {\bf r}_{3} - {\bf r}_{2} \]
\pagebreak

${\bf b}_{1}$
\pagebreak

${\bf b}_{2}$
\pagebreak

${\bf b}_{3}$
\pagebreak

$\phi = 0$
\pagebreak

$\phi = \pi $
\pagebreak

$ \phi $
\pagebreak

$ {\bf r}_{i} $
\pagebreak

\[ {\bf b}_i = {\bf r}_i - {\bf r}_{i-1} \]
\pagebreak

\[ {\bf v}_{1} = {\bf b}_1 \times {\bf b}_2 \quad\quad {\bf v}_{2} = {\bf b}_2 \times {\bf b}_3 \]
\pagebreak

\[ {\bf u}_1 = {\bf v}_{1}/|{\bf v}_{1}| \quad\quad {\bf u}_2 = {\bf v}_{2}/|{\bf v}_{2}| \]
\pagebreak

\[ \cos(\phi) \equiv {\bf u}_1 \cdot {\bf u}_2 \]
\pagebreak

$0 \leq i < 4$
\pagebreak

\[ V(\phi) = K_{0} + \sum_{m=1}^{4} K_{m} \cos(m\phi) \]
\pagebreak

\[ V(\phi) = K_{0} + \sum_{m=1}^{4} K_{m} \cos(m \phi)] \]
\pagebreak

$\rho$
\pagebreak

$\rho \equiv 0.7$
\pagebreak

$V_{i}(x)$
\pagebreak

$i$
\pagebreak

\[ V_{i}(x) = \lambda A_{i} \tanh \left ( \frac{1}{WqL} \cos( qx ) \right) \]
\pagebreak

\[ q = \frac{2\pi}{L}n \]
\pagebreak

$L$
\pagebreak

$n$
\pagebreak

$W$
\pagebreak

$A_{i}$
\pagebreak

$\lambda$
\pagebreak

$z$
\pagebreak

$0 < z < L$
\pagebreak

$z = 0$
\pagebreak

$z = L$
\pagebreak

\[ V(d) = \frac{4\pi \epsilon \rho\sigma^{3}} {45} \left ( \frac{\sigma^{9}}{d^{9}} - 7.5 \frac{\sigma^{9}}{d^{9}} + \frac{25}{\sqrt{10}} \right) \]
\pagebreak

$ d_{i} < d < d_{c} $
\pagebreak

$ d_{i} = 0.506079 \sigma $
\pagebreak

$ d_{c} $
\pagebreak

$ d > d_{c} $
\pagebreak

$ V(d) = 0 $
\pagebreak

$ d < d_{i} $
\pagebreak

$ V(d) = V(d_{i}) $
\pagebreak

\[ V(r) = \frac{\epsilon}{2} \left ( 1 - \frac{ r}{\sigma} \right )^{2} \]
\pagebreak

$ r < \sigma $
\pagebreak

$ r > \sigma $
\pagebreak

$\sigma$
\pagebreak

$j$
\pagebreak

\[ V(r) = 4 \epsilon \left [ \left ( \frac{\sigma}{r} \right )^{12} - \left ( \frac{\sigma}{r} \right )^{6} \right ] + s \]
\pagebreak

$s$
\pagebreak

$V(r_c) = 0$
\pagebreak

$r_{c}/\sigma = 1.122 = 2^{1/6}$
\pagebreak

$ r = \sigma 2^{1/6}$
\pagebreak

\[ r_{c} \equiv 2^{1/6} \sigma \]
\pagebreak

\[ V(r) = 4 \epsilon \left [ \left ( \frac{\sigma}{r} \right )^{12} - \left ( \frac{\sigma}{r} \right )^{6} + \frac{1}{4} \right ] \]
\pagebreak

\[ C(t) = k_{B}T G(t) \]
\pagebreak

$G(t)$
\pagebreak

$C(t)$
\pagebreak

\[ C(t) = \frac{1}{10} \sum_{ij=0}^{2} \langle V [\sigma_{ij}(t) - P(t)\delta_{ij}] [\sigma_{ij}(0) - P(0)\delta_{ij}] \rangle \]
\pagebreak

$V = \sqrt{V(t)V(0)}$
\pagebreak

$\sigma_{ij}(t)$
\pagebreak

\[ P(t) \equiv \sum_{i=0}^{2} \sigma_{ii}(t)/3 \]
\pagebreak

$ R_0, R_1, ...., R_{N_{i}-1} $
\pagebreak

\[ R_{g,i}^2 = \sum_j \langle | R_j - R_{cm,i} |^2 \rangle / N_i \]
\pagebreak

$ R_{cm,i} = (R_0 + R_1 + ... R_{N_{i}-1})/N_i $
\pagebreak

$ \langle \cdots \rangle $
\pagebreak

\[ S_{ij} = \sum_{a}( u_{ai}u_{aj} - \delta_{ij} ) \]
\pagebreak

$u_{ai}$
\pagebreak

${\bf u}_{a}$
\pagebreak

\[ C(t) = \sum_{i,j=0}^{2} \langle S_{ij}(t)S_{ij}(0) \rangle \]
\pagebreak

$ V(t) = R_i(t) - R_j(t) $
\pagebreak

\[ F(\tau) \equiv \langle V(t) \cdot V(t-\tau) \rangle \]
\pagebreak

$ \tau $
\pagebreak

$ \langle \cdots \rangle$
\pagebreak

$ V(t) \cdot V(t') $
\pagebreak

$ V(t) $
\pagebreak

\[ S(k) = \sum_{m} < \rho_{ma}(k) \rho_{mb}(-k) / V > \]
\pagebreak

$\rho_a(k)$
\pagebreak

\[ \rho_{ma}(k) = \sum_{i} \exp( i k \cdot r_{mi} ) \]
\pagebreak

$ \rho_{ma}(k) $
\pagebreak

$ \rho_a(k) $
\pagebreak

$ R_0, R_1, ...., R_{N-1} $
\pagebreak

\[ R_g^2 = \sum_i \langle | R_i - R_{cm} |^2 \rangle / N \]
\pagebreak

$ R_{cm} = (R_0 + R_1 + ... R_{N-1})/N $
\pagebreak

\[ S_{m}(k) = < \rho(k) \rho(-k) / V > \]
\pagebreak

$\rho(k)$
\pagebreak

\[ \rho(k) = \sum_{a} \sum_{i} v(m, a)\exp( i k \cdot r_i ) \]
\pagebreak

\[ S(k) = < \rho_a(k) \rho_b(-k) / V > \]
\pagebreak

\[ \rho_a(k) = \sum_{i} \exp( i k \cdot r_i ) \]
\pagebreak

\[ S(k,t) = \langle \psi(k,t) \psi^{*}(k,0) / V \rangle \]
\pagebreak

$V \equiv \sqrt{V(t)V(0)}$
\pagebreak

$\psi(k,t)$
\pagebreak

\[ \psi(k,t) = \sum_{i} c_{a} \exp( i k \cdot r_i ) \]
\pagebreak

$ c_{a} $
\pagebreak

$ \psi = \rho_0 - \rho_1 $
\pagebreak

\[ m\frac{d{\bf v}}{dt} = -\frac{\partial U}{\partial {\bf r}} - m\gamma {\bf v} + {\bf f}^{\rm (r)} , \]
\pagebreak

$\gamma$
\pagebreak

${\bf f}^{\rm (r)}$
\pagebreak

\begin{eqnarray*} \frac{d{\bf v}_{i}}{dt} & = & \frac{1}{m} {\bf f}_{i} - \xi {\bf v}_{i} \\ \frac{d\xi}{dt} & = & \frac{1}{ \tau_{T}^{2} } \left( \frac{T_{K}}{T_{0}} - 1 \right ) \end{eqnarray*}
\pagebreak

${\bf v}_{i}$
\pagebreak

$T_{K} = 2K/3N$
\pagebreak

$K$
\pagebreak

$N$
\pagebreak

$T_{0}$
\pagebreak

$\tau_{T}$
\pagebreak

\[ \rho(k) = \sum_{i} v(m, a)\exp( i k \cdot r_i ) \]
\pagebreak

$a$
\pagebreak

$v(m, a)$
\pagebreak

$m$
\pagebreak

\[ S(k,t) = < \psi(k,t) \psi^{*}(k,0) > / V \]
\pagebreak

\[ F(t) = k_{B}TG(t) \]
\pagebreak

$t_{i}$
\pagebreak

\[ t_i \equiv i*interval*\Delta t \]
\pagebreak

$\Delta t$
\pagebreak

$ k_{B}T G(t) $
\pagebreak

${\bf v}$
\pagebreak

\[ m\frac{d{\bf v}}{dt} = {\bf f} \]
\pagebreak

\[ {\bf f} = -\frac{\partial U}{\partial {\bf r}} - m\gamma {\bf v} + {\bf f}^{\rm (r)} , \]
\pagebreak

\begin{eqnarray*} \langle {\bf f}^{\rm (r)}\rangle & = & 0 \\ \langle {\bf f}^{\rm (r)}(t) {\bf f}^{\rm (r)}(t') \rangle & = & 2 m kT \gamma \delta (t-t') . \end{eqnarray*}
\pagebreak

${\bf v}(n)$
\pagebreak

${\bf r}(n)$
\pagebreak

\begin{eqnarray*} \overline{\bf v}(n) & = & {\bf v}(n) + {\bf f}(n) \Delta t /(2m) \\ {\bf r}(n+1) & = & {\bf r}(n) + \overline{\bf v}(n)\Delta t \\ {\bf f}(n+1) & = & {\bf f}(\;{\bf r}(n+1),\; \overline{\bf v}(n)\; ) \\ {\bf v}(n+1) & = & \overline{\bf v}(n) + {\bf f}(n+1)\Delta t /(2m) \\ \end{eqnarray*}
\pagebreak

${\bf f}$
\pagebreak

\[ {\bf f}(n+1) = {\bf f}^{\rm (pot)}(n+1) + c_{v}\overline{\bf v}(n) + c_{r}{\bf u}(n+1), \]
\pagebreak

${\bf f}^{\rm (pot)}(n+1)$
\pagebreak

${\bf r}(n+1)$
\pagebreak

$c_{v}$
\pagebreak

$c_{r}$
\pagebreak

${\bf u}$
\pagebreak

$[-1/2, 1/2]$
\pagebreak

${\bf f}(n+1)$
\pagebreak

$\overline{\bf v}(n)$
\pagebreak

\[ \overline{\bf v} (n+1) = ( 1 + c_{v} \Delta t/m )\overline{\bf v}(n) + (c_{r}\Delta t/m) {\bf u} \]
\pagebreak

$1 + c_{v}\Delta t/m = e^{-\gamma\Delta t}$
\pagebreak

\[ c_{v} = -m (1 - e^{-\gamma\Delta t})/\Delta t , \]
\pagebreak

$c_{v} < 0$
\pagebreak

\[ \langle v_{i} v_{j} \rangle = \delta_{ij} k_{B}T/m , \]
\pagebreak

\[ \langle \overline{v}_{i} \overline{v}_{j} \rangle = \delta_{ij} d k_{B}T/m . \]
\pagebreak

$d$
\pagebreak

$\gamma\Delta t \rightarrow 0$
\pagebreak

$\langle u_{i} u_{j} \rangle = \delta_{ij}/12$
\pagebreak

\[ c_{r} = \sqrt{12 m k_{B}T d ( 1 - e^{-2\gamma\Delta t})}/\Delta t \]
\pagebreak

\[ {\bf v}(n+1) = [1 + c_{v}\Delta t/(2m)] \overline{\bf v}(n) + [c_{r} \Delta t/(2m)] {\bf u}(n+1) \]
\pagebreak

\[ d = 2/(1 + e^{-\gamma\Delta t}) . \]
\pagebreak

\end{document}
